Misc cleanup

theories/trace.v
@@ -25,55 +25,56 @@ Section well_formed.
   Context {S L : Type}.
   Context (R : S → L → S → Prop).
 
-  Definition head_trace' (tr : trace_aux S L) : S * option L :=
+  Definition head_trace_aux (tr : trace_aux S L) : S * option L :=
     match tr with
     | tr_singl s => (s, None)
     | tr_cons s ℓ tr => (s, Some ℓ)
     end.
 
-  Definition head_trace : trace S L → option (S * option L) :=
-    fmap head_trace'.
-
-  Definition tail_trace' (tr : trace_aux S L) : option (trace_aux S L) :=
+  Definition tail_trace_aux (tr : trace_aux S L) : option (trace_aux S L) :=
     match tr with
     | tr_singl s => None
     | tr_cons s ℓ r => Some r
     end.
 
-  Definition tail_trace : trace S L → trace S L :=
-    mbind tail_trace'.
+  Definition head_trace : trace S L → option (S * option L) :=
+    fmap head_trace_aux.
 
-  CoInductive trace_maximal : trace S L → Prop :=
-  | trace_maximal_empty : trace_maximal None
-  | trace_maximal_singleton c :
-    (∀ oζ c', ¬ R c oζ c') → trace_maximal (Some $ tr_singl c)
-  | trace_maximal_cons c l tr c' :
+  Definition tail_trace : trace S L → trace S L :=
+    mbind tail_trace_aux.
+
+  CoInductive trace_well_formed : trace S L → Prop :=
+  | trace_well_formed_empty : trace_well_formed None
+  | trace_well_formed_singleton c :
+    (∀ oζ c', ¬ R c oζ c') → trace_well_formed (Some $ tr_singl c)
+  | trace_well_formed_cons c l tr c' :
     fst <$> head_trace (Some tr) = Some c' →
     R c l c' →
-    trace_maximal (Some tr) →
-    trace_maximal (Some $ tr_cons c l tr).
+    trace_well_formed (Some tr) →
+    trace_well_formed (Some $ tr_cons c l tr).
 
-  Lemma trace_maximal_tail tr : trace_maximal tr → trace_maximal (tail_trace tr).
+  Lemma trace_well_formed_tail tr : trace_well_formed tr → trace_well_formed (tail_trace tr).
   Proof.
-    intros wf.
-    destruct tr as [[]|].
-    - constructor.
-    - simpl. inversion wf; simplify_eq. done.
-    - simpl. constructor.
+    intros Hwf.
+    destruct tr as [[s|s l tr]|].
+    - by constructor.
+    - by inversion Hwf; simplify_eq.
+    - by constructor.
   Qed.
 
 End well_formed.
 
 Record wf_trace S L R := Trace {
   tr_car : trace S L;
-  tr_wf : trace_maximal R tr_car;
+  tr_wf : trace_well_formed R tr_car;
 }.
 
 Arguments Trace {_ _ _} _ _.
 Arguments tr_car {_ _ _} _.
 Arguments tr_wf {_ _ _} _.
-Arguments trace_maximal_empty {_ _ _}.
-Arguments trace_maximal_singleton {_ _ _} _ _.
+Arguments trace_well_formed_empty {_ _ _}.
+Arguments trace_well_formed_singleton {_ _ _} _ _.
+Arguments trace_well_formed_cons {_ _ _} _ _.
 
 Notation "tr @ tr_wf" := (Trace tr tr_wf) (at level 100).
 
@@ -84,8 +85,8 @@ Section wf_after.
   Definition wf_head (tr : wf_trace S L Rel) : option (S * option L) :=
     head_trace (tr_car tr).
 
-  Definition wf_tail : wf_trace S L Rel → wf_trace S L Rel :=
-    λ tr, (tail_trace (tr_car tr)) @ (trace_maximal_tail Rel (tr_car tr) (tr_wf tr)).
+  Definition wf_tail (tr : wf_trace S L Rel) : wf_trace S L Rel :=
+    (tail_trace (tr_car tr)) @ (trace_well_formed_tail Rel (tr_car tr) (tr_wf tr)).
 
   Notation wf_after n t := (Nat.iter n wf_tail t).
 
@@ -94,10 +95,10 @@ Section wf_after.
   Proof. induction n; [done|]. simpl. by rewrite IHn. Qed.
 
   Lemma wf_after_0 tr : wf_after 0 tr = tr.
-  Proof. by destruct tr. Qed.
+  Proof. done. Qed.
 
   Lemma wf_after_sum n m tr : wf_after (n+m) tr = wf_after n (wf_after m tr).
-  Proof. rewrite Nat.iter_add. done. Qed.
+  Proof. by rewrite Nat.iter_add. Qed.
 
   Lemma wf_tail_wf_after (tr : wf_trace S L Rel) : wf_tail tr = wf_after 1 tr.
   Proof. done. Qed.
